A ton of simplifications, but broke the proof of d2.wf_problem in the meantime.

PDDL_Normalization.thy
@@ -15,46 +15,36 @@ Some of these aren't strictly necessary and will only be kept in place for the M
 * (maybe) check action signature types for well-formedness. (domain)\<close>
 
 text \<open>Check if a formula consists of only (nested) conjunctions of literals.\<close>
-abbreviation singleton_types :: "('a \<times> type) list \<Rightarrow> bool" where
-  "singleton_types os \<equiv> (\<forall>(_, t) \<in> set os. length (primitives t) = 1)"
 
-context ast_domain
-begin
-  (* Omitting this from wf_action_schema is a little annoying for me *)
-  definition wf_action_params :: "ast_action_schema \<Rightarrow> bool" where
-    "wf_action_params a \<equiv> (\<forall>t \<in> snd ` (set (parameters a)). wf_type t)"
-  
-  definition restrict_dom :: bool where
-    "restrict_dom \<equiv> singleton_types (consts D)
-                    \<and> (\<forall>a\<in>set (actions D). wf_action_params a)"
-end
+fun single_type :: "type \<Rightarrow> bool" where
+  "single_type (Either ts) \<longleftrightarrow> length ts = 1"
+abbreviation single_types :: "('a \<times> type) list \<Rightarrow> bool" where
+  "single_types os \<equiv> \<forall>(_, T) \<in> set os. single_type T"
+
+
+(* This being omitted from wf_action_schema is a little annoying for me *)
+definition (in ast_domain) wf_action_params :: "ast_action_schema \<Rightarrow> bool" where
+  "wf_action_params a \<equiv> (\<forall>(n, t) \<in> set (parameters a). wf_type t)"
+
+definition (in ast_domain) restrict_dom :: bool where
+  "restrict_dom \<equiv> single_types (consts D)
+                  \<and> (\<forall>a\<in>set (actions D). wf_action_params a)"
+
 
 locale restr_domain = wf_ast_domain +
-  assumes restrD: restrict_dom
-begin
-  (* this is the most important and most referenced property restriction *)
-  lemma single_t_cnsts: "singleton_types (consts D)"
-    using restrD by (auto simp add: restrict_dom_def)
-end
+  assumes restrict_dom: restrict_dom
 
-context ast_problem
-begin
-  definition restrict_prob :: bool where
-    "restrict_prob \<equiv> restrict_dom
-                  \<and> singleton_types (objects P)
-                  \<and> only_conj (goal P)"
-end
+definition (in ast_problem) restrict_prob :: bool where
+  "restrict_prob \<equiv> restrict_dom
+    \<and> single_types (objects P)
+    \<and> only_conj (goal P)"
 
 locale restr_problem = wf_ast_problem +
-  assumes restrP: restrict_prob
-begin
-  sublocale restr_domain "domain P"
-    apply unfold_locales
-    using restrP restrict_prob_def by simp
+  assumes restrict_prob: restrict_prob
 
-  lemma single_t_cnsts: "singleton_types (objects P)"
-    using restrP by (auto simp add: restrict_dom_def restrict_prob_def)
-end
+sublocale restr_problem \<subseteq> restr_domain "D"
+  apply unfold_locales
+  using restrict_prob restrict_prob_def by simp
 
 subsection \<open>Type Normalization\<close>
 
@@ -82,19 +72,31 @@ begin
   definition supertype_preds :: "name \<Rightarrow> predicate list" where
     "supertype_preds t \<equiv> map pred_for_type (supertypes_of t)"
   
-  text \<open>This only works for singleton types on purpose.\<close>
+  text \<open>This only works for single types on purpose.\<close>
   fun supertype_facts_for :: "(object \<times> type) \<Rightarrow> object atom formula list" where
     "supertype_facts_for (n, Either [t]) =
       map (Atom \<circ> (\<lambda>p. predAtm p [n])) (supertype_preds t)" |
     "supertype_facts_for (n, _) = undefined"
 
-  (* TODO sugar *)
-  fun type_conds :: "type \<Rightarrow> predicate list" where
-    "type_conds t = map pred_for_type (primitives t)"
+  fun type_cond :: "variable \<Rightarrow> name \<Rightarrow> term atom formula" where
+    "type_cond v t = Atom (predAtm (pred_for_type t) [term.VAR v])"
+  fun type_precond :: "variable \<times> type \<Rightarrow> term atom formula" where
+    "type_precond (v, (Either ts)) = disj_fmlas (map (type_cond v) ts)"
+
+(**) lemma xd: "type_precond (v, (Either ts))
+  = disj_fmlas (map ((\<lambda>p. Atom (predAtm p [term.VAR v])) \<circ> pred_for_type) ts)"
+  by (smt (verit) ast_domain.type_precond.simps fun_comp_eq_conv type_cond.simps)
+
+(**) lemma xd2: "type_precond (v, (Either ts))
+  = disj_fmlas (map (Atom \<circ>(\<lambda>p. predAtm p [term.VAR v]) \<circ> pred_for_type) ts)"
+  using xd fun_comp_eq_conv by fastforce
+
+(*  fun type_conds :: "type \<Rightarrow> predicate list" where
+    "type_conds T = map pred_for_type (primitives T)"
   
   fun type_precond :: "(variable \<times> type) \<Rightarrow> term atom formula" where
     "type_precond (v, T) =
-      disj_fmlas (map (Atom \<circ> (\<lambda>p. predAtm p [term.VAR v])) (type_conds T))"
+      disj_fmlas (map (Atom \<circ> (\<lambda>p. predAtm p [term.VAR v])) (type_conds T))" *)
   
   fun param_precond :: "(variable \<times> type) list \<Rightarrow> term atom formula" where
     "param_precond params = conj_fmlas (map type_precond params)"
@@ -105,8 +107,8 @@ begin
   definition detype_preds :: "predicate_decl list \<Rightarrow> predicate_decl list" where
     "detype_preds preds \<equiv> map detype_pred preds"
 
-  abbreviation detype_ent :: "('ent \<times> type) \<Rightarrow> ('ent \<times> type)" where
-    "detype_ent ent \<equiv> (fst ent, \<omega>)"
+  fun detype_ent :: "('ent \<times> type) \<Rightarrow> ('ent \<times> type)" where
+    "detype_ent (n, T) = (n, \<omega>)"
 
   definition detype_ents :: "('ent \<times> type) list \<Rightarrow> ('ent \<times> type) list" where
     "detype_ents params \<equiv> map detype_ent params"
@@ -114,14 +116,6 @@ begin
   fun detype_ac :: "ast_action_schema \<Rightarrow> ast_action_schema" where
   "detype_ac (Action_Schema nam params pre eff) =
     Action_Schema nam (detype_ents params) (param_precond params \<^bold>\<and> pre) eff"
-  (* TODO other alternative *)
-  lemma detype_ac_def:
-    "detype_ac ac = Action_Schema
-      (ast_action_schema.name ac)
-      (detype_ents (ast_action_schema.parameters ac))
-      (param_precond (ast_action_schema.parameters ac) \<^bold>\<and> (ast_action_schema.precondition ac))
-      (ast_action_schema.effect ac)"
-    by (metis ast_action_schema.collapse detype_ac.simps)
 
   definition detype_dom :: "ast_domain" where
   "detype_dom \<equiv>
@@ -174,7 +168,6 @@ definition (in ast_problem) normalized_prob :: "bool" where
 
 
 (* ------------------------------------- PROOFS ------------------------------------------------- *)
-
 subsection \<open>Type Normalization Proofs\<close>
 
 text \<open>This is only to simplify the syntax. So I can just do
@@ -211,19 +204,59 @@ sublocale restr_problem2 \<subseteq> wf_ast_problem2
 sublocale restr_problem2 \<subseteq> restr_domain2 D
   apply unfold_locales .
 
-context ast_domain
-begin
+
+text \<open> Locale stuff \<close>
+
+  (* just restrict_dom unfolded *)
+  lemma (in restr_domain) restr_D: "single_types (consts D)" "(\<forall>a\<in>set (actions D). wf_action_params a)"
+    using restrict_dom restrict_dom_def by auto
+  
+  (* just restrict_prob unfolded *)
+  lemma (in restr_problem) restr_P: "single_types (objects P)" "only_conj (goal P)"
+    using restrict_prob restrict_prob_def by auto
+  
+  lemma (in restr_problem) single_t_objs: "single_types (consts D @ objects P)"
+    using restr_D restr_P by auto
+
+  (* wf_domain unfolded and split *)
+  lemmas (in wf_ast_domain) wf_D = conj_split_7[OF wf_domain[unfolded wf_domain_def]]
+
+  (* wf_problem unfolded and split, but omitting the first fact "wf_domain" *)
+  lemmas (in wf_ast_problem) wf_P =
+    conj_split_5[OF wf_problem[unfolded wf_problem_def, THEN conjunct2]]
+
+  lemmas (in wf_ast_problem) wf_DP = wf_D wf_P
 
 text \<open> basic stuff \<close>
 
   lemma (in -) dist_pred: "distinct names \<longleftrightarrow> distinct (map Pred names)"
     by (meson distinct_map inj_onI predicate.inject)
 
-  lemmas (in wf_ast_domain) wf_dom_def = wf_domain[unfolded wf_domain_def]
-  
-  lemmas (in wf_ast_problem) wf_prob_def = wf_problem[unfolded wf_problem_def]
+  lemma (in wf_ast_problem) objT_Some: "(n, T) \<in> set (consts D @ objects P) \<longleftrightarrow> objT n = Some T"
+  proof -
+    have "distinct (map fst (consts D @ objects P))"
+      using wf_P(1) by auto
+    thus ?thesis using objT_alt
+      by (metis map_of_eq_Some_iff)
+  qed
+
+  lemma (in wf_ast_problem) cnst_obj_ids_disj:
+    "fst ` set (consts D) \<inter> fst ` set (objects P) = {}"
+    using list.set_map wf_P(1) by auto
+
+  lemma (in wf_ast_problem) objm_le_objT: "map_of (objects P) \<subseteq>\<^sub>m objT"
+  proof -
+    have "dom constT \<inter> dom (map_of (objects P)) = {}"
+      using constT_def cnst_obj_ids_disj
+      by (simp add: dom_map_of_conv_image_fst)
+    thus ?thesis using objT_def
+      by (simp add: map_add_comm map_le_iff_map_add_commute)  
+  qed
 
 text \<open> type system \<close>
+
+context ast_domain
+begin
 
   lemma (in -) wf_object: "ast_domain.wf_type d \<omega>"
     unfolding ast_domain.wf_type.simps by simp
@@ -242,6 +275,7 @@ text \<open> type system \<close>
     apply (split term.split)
     by simp
 
+  (* TODO: improve this to _eq_Some_iff *)
   lemma tyterm_elem: "(ty_term (map_of varT) (map_of cnstT) x \<noteq> None)
     \<longleftrightarrow> (case x of term.VAR x' \<Rightarrow> x' \<in> fst ` set varT |
                    term.CONST x' \<Rightarrow> x' \<in> fst ` set cnstT)"
@@ -250,13 +284,11 @@ text \<open> type system \<close>
 
 text \<open> type_names \<close>
 
- lemma wf_type_iff_listed: "wf_type T \<longleftrightarrow> (\<forall>t \<in> set (primitives T). t \<in> set (type_names))"
-  proof -
-    have "set type_names = insert ''object'' (fst ` set (types D))"  by auto
-    hence "wf_type (Either ts) \<longleftrightarrow> (\<forall>t \<in> set ts. t \<in> set (type_names))" for ts
-      by (simp add: subset_code(1))
-    thus ?thesis using type.collapse by metis
-  qed
+  lemma type_names_set[simp]: "set type_names = insert ''object'' (fst ` set (types D))"
+    by auto
+
+  lemma wf_type_iff_listed: "wf_type (Either ts) \<longleftrightarrow> (set ts \<subseteq> set (type_names))"
+    using type_names_set by simp
 
 text \<open> pred_for_type \<close>
 
@@ -270,21 +302,18 @@ text \<open> pred_for_type \<close>
     thus ?thesis by auto
   qed
 
+  lemma pred_for_type_inj: "inj pred_for_type" using inj_def by auto
+
+  lemma pred_for_type_dis:
+    assumes "distinct ts"
+    shows "distinct (map pred_for_type ts)"
+    using assms pred_for_type_inj by (rule map_inj_dis)
+
 text \<open> type_preds \<close>
 
-  lemma tps_dis:
+  lemma type_preds_dis:
     "distinct (map pred type_preds)" (is "distinct ?tp_ids")
-  proof -
-    let ?pred_ids = "map pred (predicates D)"
-    let ?prefix = "safe_prefix (map predicate.name ?pred_ids)"
-    have tp_ids: "?tp_ids = map (Pred \<circ> ((@) ?prefix)) type_names"
-        by (simp add: type_preds_ids)
-    have "distinct (map ((@) ?prefix) type_names)" (* because: distinct type_names *)
-      using dist_prefix by simp
-    hence "distinct (map (Pred \<circ> ((@) ?prefix)) type_names)"
-      using dist_pred by simp
-    thus "distinct ?tp_ids" using tp_ids by metis
-  qed
+    using pred_for_type_dis type_preds_ids by force
 
 text \<open> supertype preds \<close>
 
@@ -298,40 +327,28 @@ text \<open> detyped preds \<close>
     "\<forall>p \<in> set (predicates D2). \<forall>T \<in> set (argTs p). T = \<omega>"
     using type_preds_def detype_preds_def detype_dom_def by auto
 
-  lemma dt_pred_name: "pred (detype_pred pd) = pred pd" by simp
+  lemma dt_pred_id: "pred (detype_pred pd) = pred pd" by simp
 
-  lemma dt_preds_names:
+  lemma dt_preds_ids:
     "map pred (detype_preds ps) = map pred ps"
-    using dt_pred_name detype_preds_def by simp
+    using dt_pred_id detype_preds_def by simp
 
-  (* TODO simplify *)
+  lemma type_pred_notin: "pred_for_type t \<notin> pred ` set (predicates D)"
+  proof -
+    have "predicate.name (pred_for_type t) \<notin> set pred_names"
+      using safe_prefix_correct predicate.sel by presburger
+    thus ?thesis by force
+  qed
+
   lemma tps_dt_preds_disj:
     "pred ` set type_preds \<inter> pred ` set (detype_preds (predicates D)) = {}"
   proof -
-    let ?preds = "map pred (predicates D)"
-    let ?t_preds = "map pred type_preds"
-    let ?dt_preds = "map pred (detype_preds (predicates D))"
-
-    let ?prefix = "safe_prefix (map predicate.name ?preds)"
-    (* =  map (pred_for_type D) (type_names D) *)
-    have t_ps_expand: "?t_preds = map (Pred \<circ> ((@) ?prefix)) type_names"
-      by (simp add: type_preds_def)
-    (* define, not let, because the terms become too big for the solver *)
-    define pnames where "pnames \<equiv> map predicate.name ?preds"
-    define tp_names where "tp_names \<equiv> map (((@) (safe_prefix pnames))) type_names"
-    
-    have "set (map ((@) (safe_prefix pnames)) type_names) \<inter> set pnames = {}"
-      using safe_prefix_correct by auto
-    hence "set tp_names \<inter> set pnames = {}" using tp_names_def pnames_def by simp
-    hence "set (map Pred tp_names) \<inter> set (map Pred pnames) = {}" by auto
-    hence "set (map (Pred \<circ> ((@) (safe_prefix pnames))) type_names) \<inter> set (map Pred pnames) = {}"
-      using tp_names_def by (metis map_map)
-  
-    moreover have "map Pred pnames = ?preds" using pnames_def by simp
-    moreover have "?t_preds = map (Pred \<circ> ((@) (safe_prefix pnames))) type_names"
-      using t_ps_expand pnames_def by blast
-    ultimately have g2: "set ?t_preds \<inter> set ?dt_preds = {}" by (metis dt_preds_names)
-    thus ?thesis by simp
+    have "pred ` set type_preds = pred_for_type ` set type_names"
+      by (metis type_preds_ids list.set_map)
+    moreover have "pred ` set (detype_preds (predicates D)) = pred ` set (predicates D)"
+      using dt_preds_ids by (metis list.set_map)
+    ultimately show ?thesis using type_pred_notin
+      by (metis disjoint_iff_not_equal type_pred_refs_type)
   qed
 
   lemma (in wf_ast_domain) t_preds_dis:
@@ -341,29 +358,21 @@ text \<open> detyped preds \<close>
        and the additional predicate names are unique (based on unique type names)
        and distinct from the original predicates. *)
 
-    have c1: "distinct (map pred (detype_preds (predicates D)))"
-      using dt_preds_names wf_dom_def by simp
-    note c2 = tps_dt_preds_disj
-    note c3 = tps_dis
-  
-    from c1 c2 c3 have "distinct (map pred (type_preds @ detype_preds (predicates D)))" by simp
-    thus ?thesis using ast_domain.sel(2) detype_dom_def by presburger
+    have "distinct (map pred (detype_preds (predicates D)))"
+      using dt_preds_ids wf_D(2) by simp
+    hence "distinct (map pred (type_preds @ detype_preds (predicates D)))"
+      using tps_dt_preds_disj type_preds_dis by simp
+    thus ?thesis using detype_dom_def by simp
   qed
 
   lemma (in ast_domain2) t_preds_wf:
-    "\<forall>p \<in> set (predicates D2). d2.wf_predicate_decl p"
-  proof -
-    have "\<forall>p \<in> set (predicates D2). \<forall>T \<in> set (argTs p). T = \<omega>"
-      by (rule preds_detyped)
-    hence "\<forall>p \<in> set (predicates D2). \<forall>T \<in> set (argTs p). d2.wf_type T"
-      using preds_detyped wf_object by auto
-    thus ?thesis by (metis d2.wf_predicate_decl.simps predicate_decl.collapse)
-  qed
+    "p \<in> set (predicates D2) \<longrightarrow> d2.wf_predicate_decl p"
+    apply (cases p) using preds_detyped wf_object by auto
 
 text \<open> detype ents \<close>
 
   lemma ents_detyped: "\<forall>(n, T) \<in> set (detype_ents ents). T = \<omega>"
-    by (simp add: detype_ents_def case_prod_beta' detype_dom_def)
+    by (auto simp add: detype_ents_def)
 
   lemma t_ents_names:
     "map fst (detype_ents ents) = map fst ents"
@@ -383,12 +392,10 @@ text \<open> detype ents \<close>
   lemma t_entT_Some:
     shows "map_of ents x \<noteq> None \<longleftrightarrow> map_of (detype_ents ents) x = Some \<omega>"
   proof -
-    have 1: "\<forall>T \<in> snd ` set (detype_ents ents). T = \<omega>" using ents_detyped by fastforce
     have "map_of ents x \<noteq> None \<longleftrightarrow> x \<in> fst ` set ents" using map_of_eq_None_iff by metis
     also have "... \<longleftrightarrow> x \<in> fst ` set (detype_ents ents)" using t_ents_names by (metis list.set_map)
-    
-    ultimately show ?thesis using 1 map_of_in_R_iff
-      by (metis map_of_eq_None_iff option.discI)
+    ultimately show ?thesis using map_of_single_val[OF ents_detyped]
+      by metis
   qed
 
   lemma t_entT_None:
@@ -398,33 +405,77 @@ text \<open> detype ents \<close>
 text \<open> predicate signatures \<open>sig\<close> \<close>
 
   abbreviation "split_pred \<equiv> (\<lambda>PredDecl p n \<Rightarrow> (p, n))"
+  
+  lemma split_pred_alt: "split_pred p = (pred p, argTs p)"
+    using predicate_decl.case_eq_if by auto
 
-  lemma pred_resolve:
+  lemma (in ast_domain) pred_resolve:
     assumes "distinct (map pred preds)"
-    shows "map_of (map split_pred preds) p = Some Ts
-      \<longleftrightarrow> PredDecl p Ts \<in> set preds"
+    shows "map_of (map split_pred preds) p = Some Ts \<longleftrightarrow> PredDecl p Ts \<in> set preds"
   proof -
-    let ?pred_map = "map split_pred preds"
-    have fst_split: "fst \<circ> split_pred = pred"
-      by (simp add: comp_def predicate_decl.case_eq_if)
-    hence "distinct (map fst ?pred_map)" using assms by simp
-    hence 1: "map_of ?pred_map p = Some Ts \<longleftrightarrow> (p, Ts) \<in> set ?pred_map" by simp
-
-    (* this direction seems to be harder to infer automatically *)
-    moreover have "\<And>pred. split_pred pred = (p, Ts) \<Longrightarrow> pred = PredDecl p Ts"
-      by (metis predicate_decl.case predicate_decl.exhaust prod.inject)
-    hence "(p, Ts) \<in> set ?pred_map \<longleftrightarrow> PredDecl p Ts \<in> set preds"
-      by force
-    thus ?thesis using 1 by presburger
+    have "map (fst \<circ> split_pred) preds = map pred preds"
+      using split_pred_alt by simp
+    hence dis: "distinct (map (fst \<circ> split_pred) preds)"
+      using assms by metis
+  
+    have "PredDecl p Ts \<in> set preds
+      \<longleftrightarrow> (p, Ts) \<in> set (map split_pred preds)"
+      using split_pred_alt by force
+    also have "... \<longleftrightarrow> map_of (map split_pred preds) p = Some Ts"
+      using sig_def dis by simp
+  
+    ultimately show ?thesis by simp
   qed
 
-  lemma (in wf_ast_domain) sig_some:
+  lemma (in wf_ast_domain) sig_Some:
     "sig p = Some Ts \<longleftrightarrow> PredDecl p Ts \<in> set (predicates D)"
+    using wf_D(2) pred_resolve sig_def by auto
+
+  lemma (in wf_ast_domain2) sig2_aux:
+    "d2.sig p = Some Ts \<longleftrightarrow> PredDecl p Ts \<in> set type_preds \<union> set (detype_preds (predicates D))"
+    using t_preds_dis detype_dom_def pred_resolve d2.sig_def
+    by (metis ast_domain.sel(2) set_union_code)
+
+  lemma (in wf_ast_domain2) sig2_of_typepred:
+    assumes "p \<in> pred ` set type_preds"
+    shows "d2.sig p = Some [\<omega>]"
   proof -
-    have "distinct (map pred (predicates D))" using wf_dom_def by simp
-    thus ?thesis using pred_resolve sig_def by simp
+    from assms obtain Ts where pd: "PredDecl p Ts \<in> set type_preds"
+      by (metis image_iff predicate_decl.collapse)
+    hence "PredDecl p Ts \<notin> set (detype_preds (predicates D))"
+      using tps_dt_preds_disj by auto
+    moreover have "Ts = [\<omega>]" using type_preds_def pd by auto
+    ultimately show ?thesis using assms sig2_aux pd by blast
   qed
 
+  lemma (in wf_ast_domain2) type_pred_sig:
+    assumes "t \<in> set type_names"
+    shows "d2.sig (pred_for_type t) = Some [\<omega>]"
+  proof -
+    let ?p = "pred_for_type t"
+    from assms obtain Ts where pd: "PredDecl ?p Ts \<in> set type_preds"
+      using type_preds_def by auto
+    hence "PredDecl ?p Ts \<notin> set (detype_preds (predicates D))"
+      using tps_dt_preds_disj by auto
+    moreover have "Ts = [\<omega>]" using type_preds_def pd by auto
+    ultimately show ?thesis using assms sig2_aux pd by blast
+  qed
+
+
+  lemma (in wf_ast_domain2) dt_preds_arity:
+    assumes "sig p = Some Ts"
+    shows "d2.sig p = Some (replicate (length Ts) \<omega>)"
+  proof -
+    from assms have "PredDecl p Ts \<in> set (predicates D)"
+      by (simp add: sig_Some)
+    hence 1: "PredDecl p (replicate (length Ts) \<omega>) \<in> set (detype_preds (predicates D))"
+      using detype_preds_def by force
+    hence "PredDecl p (replicate (length Ts) \<omega>) \<notin> set type_preds"
+      using tps_dt_preds_disj by auto
+    thus ?thesis using sig2_aux 1 by auto
+  qed
+
+(*
   text \<open>Decompose the signature function of the detyped domain in two ways, since the domains
     are disjoint. Yes this is the best way I could think of.\<close>
   lemma (in ast_domain2) t_sig_split_a:
@@ -436,10 +487,8 @@ text \<open> predicate signatures \<open>sig\<close> \<close>
     let ?dt_pred_map = "map split_pred (detype_preds (predicates D))"
 
     (* d2.sig in terms of map1 ++ map2 *)
-    have "d2.sig = map_of ?pred_map2"
-      by (simp add: d2.sig_def)
-    also have "... = map_of (map split_pred (type_preds @ (detype_preds (predicates D))))"
-      using detype_dom_def by simp
+    have "d2.sig = map_of (map split_pred (type_preds @ (detype_preds (predicates D))))"
+      using detype_dom_def d2.sig_def by simp
     also have "... = map_of (?t_pred_map @ ?dt_pred_map)"
       by simp
     also have "... = map_of ?dt_pred_map ++ map_of ?t_pred_map" by simp
@@ -451,7 +500,7 @@ text \<open> predicate signatures \<open>sig\<close> \<close>
     "d2.sig =
       map_of (map split_pred type_preds) ++ map_of (map split_pred (detype_preds (predicates D)))"
   proof -
-    have dis: "distinct (map pred (predicates D))" using wf_dom_def by simp
+    have dis: "distinct (map pred (predicates D))" using wf_D by simp
 
     let ?pred_map2 = "(map split_pred (predicates D2))"
     let ?t_pred_map = "map split_pred type_preds"
@@ -462,9 +511,9 @@ text \<open> predicate signatures \<open>sig\<close> \<close>
     hence
       "map fst ?t_pred_map = map pred type_preds" and      
       "map fst ?dt_pred_map = map pred (predicates D)"
-      using dt_preds_names by simp_all
+      using dt_preds_ids by simp_all
     hence "fst ` set ?t_pred_map \<inter> fst ` set ?dt_pred_map = {}"
-      by (metis tps_dt_preds_disj dt_preds_names list.set_map)
+      by (metis tps_dt_preds_disj dt_preds_ids list.set_map)
     hence comm: "map_of ?t_pred_map ++ map_of ?dt_pred_map = map_of ?dt_pred_map ++ map_of ?t_pred_map"
       using map_add_comm by (metis dom_map_of_conv_image_fst)
     thus ?thesis using t_sig_split_a by simp
@@ -475,7 +524,7 @@ text \<open> predicate signatures \<open>sig\<close> \<close>
       (p \<in> pred ` set (predicates D))
       \<or> (p \<in> pred_for_type ` set type_names)"
   proof -
-    have dis: "distinct (map pred (predicates D))" using wf_dom_def by simp
+    have dis: "distinct (map pred (predicates D))" using wf_D by simp
 
     let ?pred_map2 = "(map split_pred (predicates D2))"
     let ?t_pred_map = "map split_pred type_preds"
@@ -492,7 +541,7 @@ text \<open> predicate signatures \<open>sig\<close> \<close>
     hence
       a: "map fst ?t_pred_map = map pred_for_type type_names" and      
       b: "map fst ?dt_pred_map = map pred (predicates D)"
-      using type_preds_ids dt_preds_names by simp_all
+      using type_preds_ids dt_preds_ids by simp_all
     hence
       "fst ` set ?t_pred_map = pred_for_type ` set type_names" and
       "fst ` set ?dt_pred_map = pred ` set (predicates D)"
@@ -506,17 +555,30 @@ text \<open> predicate signatures \<open>sig\<close> \<close>
     assumes "sig p = Some Ts"
     shows "d2.sig p = Some (replicate (length Ts) \<omega>)"
   proof -
-    have dis: "distinct (map pred (predicates D))" using wf_dom_def by simp
+    have dis: "distinct (map pred (predicates D))" using wf_D by simp
     let ?dt_pred_map = "map split_pred (detype_preds (predicates D))"
 
     have "PredDecl p Ts \<in> set (predicates D)" using assms sig_some by simp
     hence "PredDecl p (replicate (length Ts) \<omega>) \<in> set (detype_preds (predicates D))"
       using detype_preds_def by force
     hence "map_of ?dt_pred_map p = Some (replicate (length Ts) \<omega>)" using pred_resolve
-      using dis dt_preds_names by force
+      using dis dt_preds_ids by force
     thus ?thesis using t_sig_split_b by simp
-  qed
+  qed 
 
+(* type pred sigs *)
+
+  lemma (in wf_ast_domain2) type_pred_sig:
+    assumes "t \<in> set type_names"
+    shows "d2.sig (pred_for_type t) = Some [\<omega>]"
+
+    using assms sig2_of_typepred type_preds_def
+  proof -
+    have "PredDecl (pred_for_type t) [\<omega>] \<in> set (predicates D2)"
+      using type_preds_def assms detype_dom_def by fastforce
+    thus ?thesis using detype_dom_def
+      by (metis d2.sig_def pred_resolve t_preds_dis)
+  qed *)
 
 text \<open> type maps \<close>
 
@@ -526,19 +588,44 @@ text \<open> type maps \<close>
   lemma (in ast_domain2) t_constT_None: "constT c = None \<longleftrightarrow> d2.constT c = None"
     using t_entT_None ast_domain.constT_def detype_dom_def by fastforce
 
+  (* lemma "distinct ((map fst m) @ (map fst n)) \<Longrightarrow> map_of m ++ map_of n = map_of n ++ map_of m"
+    by (metis distinct_append dom_map_of_conv_image_fst list.set_map map_add_comm)
+
+  lemma "map_of m ++ map_of n = map_of (n @ m)"
+    by simp *)
+
+  lemma (in ast_problem2) t_cnsts_objs_names: "map fst (consts D @ objects P)
+    = map fst (detype_ents (consts D) @ detype_ents (objects P))"
+    using t_ents_names by (metis map_append)
+
+  lemma (in wf_ast_problem2) t_objm_le_objT:
+    "map_of (objects P2) \<subseteq>\<^sub>m p2.objT"
+  proof -
+    have "distinct (map fst (consts D @ objects P))" using wf_P(1) by auto
+    hence "distinct (map fst (consts D2 @ objects P2))" using t_cnsts_objs_names
+      detype_dom_def detype_prob_def by (metis ast_domain.sel(3) ast_problem.sel(2))
+    hence "fst ` set (objects P2) \<inter> fst ` set (consts D2) = {}"
+      by auto
+    hence "dom (map_of (objects P2)) \<inter> dom d2.constT = {}" using d2.constT_def
+      by (simp add: dom_map_of_conv_image_fst)
+    thus ?thesis using map_add_comm p2.objT_def
+      by (metis ast_problem.sel(1) detype_prob_def map_le_iff_map_add_commute)
+  qed
+
+  lemma (in ast_problem2) "p2.constT \<subseteq>\<^sub>m p2.objT"
+    by (rule p2.constT_ss_objT)
+
   lemma (in ast_problem2) t_objT_Some: "objT c \<noteq> None \<longleftrightarrow> p2.objT c = Some \<omega>"
   proof -
-    have "objT c \<noteq> None \<longleftrightarrow> constT c \<noteq> None \<or> constT c = None \<and> map_of (objects P) c \<noteq> None"
-      using objT_def by auto
-    also have "... \<longleftrightarrow> constT c \<noteq> None \<or> constT c = None \<and> map_of (objects detype_prob) c = Some \<omega>"
-      using detype_prob_def t_entT_Some by fastforce
-    also have "... \<longleftrightarrow> p2.constT c = Some \<omega> \<or> constT c = None \<and> map_of (objects detype_prob) c = Some \<omega>"
-      using detype_prob_def t_constT_Some by fastforce
-    also have "... \<longleftrightarrow> p2.constT c = Some \<omega> \<or> p2.constT c = None \<and> map_of (objects detype_prob) c = Some \<omega>"
-      using detype_prob_def t_constT_None by fastforce
-    also have "... \<longleftrightarrow> (map_of (objects detype_prob) ++ p2.constT) c = Some \<omega>"
-      using map_add_Some_iff by fastforce
-    also have "... \<longleftrightarrow> p2.objT c = Some \<omega>" using p2.objT_def by simp
+    have 1: "\<forall>(x, y) \<in> set (detype_ents (consts D) @ detype_ents (objects P)). y = \<omega>"
+      using ents_detyped by fastforce
+    have "objT c \<noteq> None \<longleftrightarrow> c \<in> fst ` set (consts D @ objects P)" using t_cnsts_objs_names
+      by (metis objT_alt map_of_eq_None_iff)
+    also have "... \<longleftrightarrow> c \<in> fst ` set (detype_ents (consts D) @ detype_ents (objects P))"
+      using t_cnsts_objs_names by (metis image_set)
+    also have "... \<longleftrightarrow> p2.objT c = Some \<omega>" using map_of_single_val[OF 1]
+      using p2.objT_alt
+      by (simp add: detype_dom_def detype_prob_def)
     ultimately show ?thesis by simp
   qed
 
@@ -611,7 +698,7 @@ text \<open> formulas \<close>
     let ?os = "replicate (length Ts) \<omega>"
     from assms 1 have a: "list_all2 (d2.is_of_type tyt2) params ?os"
       by (simp add: t_tyt_params)
-    have b: "d2.sig p = Some ?os" using sigp by (simp add: t_preds_arity)
+    have b: "d2.sig p = Some ?os" using sigp by (simp add: dt_preds_arity)
 
     from a b show ?case by simp
   qed simp
@@ -639,8 +726,7 @@ text \<open> formulas \<close>
     "wf_effect tyt \<epsilon> \<longleftrightarrow>
        (\<forall>ae\<in>set (adds \<epsilon>). wf_fmla_atom tyt ae)
        \<and> (\<forall>de\<in>set (dels \<epsilon>).  wf_fmla_atom tyt de)"
-    using wf_effect.simps ast_effect.collapse
-    by metis (* TODO how to just manipulate this lemma with options? *)
+    apply (cases \<epsilon>) by simp
 
   lemma (in wf_ast_domain2) t_eff_wf:
     assumes "\<forall>e. tyt e \<noteq> None \<longrightarrow> tyt2 e = Some \<omega>"
@@ -664,25 +750,22 @@ text \<open> formulas \<close>
 
 text \<open> detype ac \<close>
 
-  lemma ac_params_detyped:
-    "\<forall>ac \<in> set (actions D2). \<forall>(n, T) \<in> set (parameters ac). T = \<omega>"
-    using detype_dom_def detype_ac_def ents_detyped by fastforce
-
   abbreviation "ac_name \<equiv> ast_action_schema.name"
   (* abbreviation (in ast_domain) "ac_params \<equiv> ast_action_schema.parameters" \<comment> just use \<open>parameters\<close> *)
   abbreviation "ac_pre \<equiv> ast_action_schema.precondition"
   abbreviation "ac_eff \<equiv> ast_action_schema.effect"
 
-  lemma t_ac_name: "ac_name (detype_ac ac) = ac_name ac"
-    by (simp add: detype_ac_def)
-  lemma t_acs_names: "map ac_name (map detype_ac acs) = map ac_name acs"
-    by (simp add: t_ac_name)
-  lemma (in wf_ast_domain) t_acs_dis:
-    "distinct (map ac_name (map detype_ac (actions D)))"
-    using t_acs_names wf_dom_def by metis
+  (* TODO just manipulate lemma *)
+  lemma detype_ac_alt:
+    "detype_ac ac = Action_Schema
+      (ac_name ac)
+      (detype_ents (parameters ac))
+      (param_precond (parameters ac) \<^bold>\<and> (ac_pre ac))
+      (ac_eff ac)"
+    apply (cases ac) by simp
 
-  (* TODO just manipulate lemma  *)
-  lemma wf_ac_expanded:
+  (* TODO just manipulate lemma *)
+  lemma wf_ac_alt:
     "wf_action_schema a \<longleftrightarrow> (
       let
         tyt = ty_term (map_of (parameters a)) constT
@@ -690,78 +773,92 @@ text \<open> detype ac \<close>
         distinct (map fst (parameters a))
       \<and> wf_fmla tyt (ac_pre a)
       \<and> wf_effect tyt (ac_eff a))"
-    using wf_action_schema.simps
-    by (metis ast_action_schema.collapse)
+    apply (cases a) by simp
+
+  lemma ac_params_detyped:
+    "\<forall>ac \<in> set (actions D2). \<forall>(n, T) \<in> set (parameters ac). T = \<omega>"
+    using detype_dom_def detype_ac_alt ents_detyped by fastforce
+
+  lemma t_ac_name: "ac_name (detype_ac ac) = ac_name ac"
+    by (simp add: detype_ac_alt)
+  lemma t_acs_names: "map ac_name (map detype_ac acs) = map ac_name acs"
+    by (simp add: t_ac_name)
+  lemma (in wf_ast_domain) t_acs_dis:
+    "distinct (map ac_name (map detype_ac (actions D)))"
+    using t_acs_names wf_D by metis
 
   lemma (in ast_domain2) t_ac_tyt:
     assumes "ty_term (map_of (parameters a)) constT x \<noteq> None"
     shows "ty_term (map_of (parameters (detype_ac a))) d2.constT x = Some \<omega>"
-    using assms detype_ac_def detype_dom_def t_tyt_Some ast_domain.constT_def by auto
+    using assms detype_ac_alt detype_dom_def t_tyt_Some ast_domain.constT_def by auto
 
   lemma params_ts_wf:
-    assumes "wf_action_params a" "p \<in> set (parameters a)"
-    shows "wf_type (snd p)"
-    using assms wf_action_params_def by blast
+    assumes "wf_action_params a" "(n, T) \<in> set (parameters a)"
+    shows "wf_type T"
+    using assms wf_action_params_def by auto
 
   lemma params_ts_exist: (* somehow this isn't trivial for the solver *)
-    assumes "wf_action_params a" "p \<in> set (parameters a)"
-    shows "\<forall>t \<in> set (primitives (snd p)). t \<in> insert ''object'' (set type_names)"
-    using assms params_ts_wf
-    by (metis wf_type_iff_listed insertI2)
+    assumes "wf_action_params a" "(n, Either ts) \<in> set (parameters a)"
+    shows "set ts \<subseteq> set type_names"
+    using assms params_ts_wf wf_type_iff_listed by blast
 
+  lemma (in wf_ast_domain2) type_cond_wf:
+    assumes "t \<in> set type_names" "tyt (term.VAR n) = Some \<omega>"
+    shows "d2.wf_fmla tyt (type_cond n t)"
+  proof -
+    from assms(1) have "d2.sig (pred_for_type t) = Some [\<omega>]" by (rule type_pred_sig)
+    hence "d2.wf_fmla tyt (Atom (predAtm (pred_for_type t) [term.VAR n]))"
+      using assms(2) d2.of_type_refl d2.is_of_type_def by fastforce
+    thus ?thesis by simp
+  qed
+
+  text \<open>
+  1. tyt p = Some T
+  2. tyt2 p = Some \<omega>
+  for every type in T, the type_cond is wf:
+    - the corresponding type_pred exists and has signature [\<omega>]
+    - the arguments are just the variable [v], due to 2 with signatures [\<omega>]
+  \<close>
   lemma (in wf_ast_domain2) type_precond_wf: (* TODO simplify if possible *)
     assumes "wf_action_params a" "p \<in> set (parameters a)"
     shows "d2.wf_fmla
       (ty_term (map_of (parameters (detype_ac a))) cnstT)
       (type_precond p)"
   proof -
+    (* type_precond.cases? *)
+    obtain n ts where p: "p = (n, Either ts)" using type_precond.cases by blast
     let ?tyt = "ty_term (map_of (parameters a)) cnstT"
     let ?tyt2 = "ty_term (map_of (parameters (detype_ac a))) cnstT"
-
-    have "?tyt (term.VAR (fst p)) \<noteq> None" using assms detype_ac_def
-      by (metis imageI map_of_eq_None_iff ty_term.simps(1))
-    hence 1: "?tyt2 (term.VAR (fst p)) = Some \<omega>" using t_tyt_var_Some
-      by (simp add: detype_ac_def)
-
-    have "\<forall>t \<in> set (primitives (snd p)). d2.wf_fmla ?tyt2 (Atom (predAtm (pred_for_type t) [term.VAR (fst p)]))"
-    proof
-      fix t assume t: "t \<in> set (primitives (snd p))"
-      have "t \<in> insert ''object'' (set type_names)" using assms params_ts_exist t by simp
-      hence "PredDecl (pred_for_type t) [\<omega>] \<in> set type_preds" using type_preds_def by fastforce
-      moreover have "set type_preds \<subseteq> set (predicates D2)" using detype_dom_def by simp
-      ultimately have "PredDecl (pred_for_type t) [\<omega>] \<in> set (predicates D2)" by auto
-      hence 2: "d2.sig (pred_for_type t) = Some [\<omega>]" using detype_dom_def
-        by (metis d2.sig_def pred_resolve t_preds_dis) (* not true outside of restr_dom because action params need not wf *)
-      from 1 2 show "d2.wf_fmla ?tyt2 (Atom (predAtm (pred_for_type t) [term.VAR (fst p)]))"
-        using d2.of_type_refl d2.is_of_type_def by fastforce
-    qed
-
-    hence "\<forall>\<phi> \<in> set (map (Atom \<circ> (\<lambda>pn. predAtm pn [term.VAR (fst p)])) (type_conds (snd p))). d2.wf_fmla ?tyt2 \<phi>"
+    
+    (* Not generally "Some (Either ts)", unless we assume wf_action_schema,
+       because param names may not be distinct. *) 
+    have "?tyt (term.VAR n) \<noteq> None" using assms detype_ac_alt
+      by (simp add: p weak_map_of_SomeI)
+    hence "?tyt2 (term.VAR n) = Some \<omega>" using t_tyt_var_Some
+      by (simp add: detype_ac_alt)
+    hence "\<forall>t \<in> set ts. d2.wf_fmla ?tyt2 (type_cond n t)"
+      using assms p type_cond_wf params_ts_exist by blast
+    hence "\<forall>\<phi> \<in> set (map (type_cond n) ts). d2.wf_fmla ?tyt2 \<phi>"
       by simp
-    hence "d2.wf_fmla ?tyt2 (disj_fmlas (map (Atom \<circ> (\<lambda>pn. predAtm pn [term.VAR (fst p)])) (type_conds (snd p))))"
-      using d2.disj_fmlas_wf by metis
-    thus "d2.wf_fmla ?tyt2 (type_precond p)"
-      by (metis prod.collapse type_precond.simps)
+    hence "d2.wf_fmla ?tyt2 (type_precond (n, Either ts))"
+      using d2.disj_fmlas_wf type_precond.simps by metis
+    thus ?thesis using p by simp
   qed
 
   lemma (in wf_ast_domain2) t_param_precond_wf:
     assumes "wf_action_params a"
     shows "d2.wf_fmla
-    (ty_term (map_of (parameters (detype_ac a))) egal)
+    (ty_term (map_of (parameters (detype_ac a))) cnstT)
     (param_precond (parameters a))"
   proof -
-    let ?tyt2 = "ty_term (map_of (parameters (detype_ac a))) egal"
-    have "param_precond (parameters a) = conj_fmlas (map type_precond (parameters a))"
-      by simp
-    have "\<forall>p \<in> set (parameters a). d2.wf_fmla
-      ?tyt2
-      (type_precond p)" using type_precond_wf assms by simp
+    let ?tyt2 = "ty_term (map_of (parameters (detype_ac a))) cnstT"
+    have "\<forall>p \<in> set (parameters a). d2.wf_fmla ?tyt2 (type_precond p)"
+      using type_precond_wf assms by simp
     hence "\<forall>\<phi> \<in> set (map type_precond (parameters a)). d2.wf_fmla ?tyt2 \<phi>" by simp
-    hence "d2.wf_fmla ?tyt2 (conj_fmlas (map type_precond (parameters a)))"
-      using d2.conj_fmlas_wf by blast
-    thus ?thesis by simp
+    thus ?thesis using d2.conj_fmlas_wf param_precond.simps by metis
   qed
 
+  text \<open>Three conditions: 1. distinct parameter names, 2. wf precondition, 3. wf effect\<close>
   lemma (in restr_domain2) t_ac_wf:
     assumes "a \<in> set (actions D)"
     shows "d2.wf_action_schema (detype_ac a)"
@@ -769,41 +866,252 @@ text \<open> detype ac \<close>
     let ?a2 = "detype_ac a"
     let ?tyt = "ty_term (map_of (parameters a)) constT"
     let ?tyt2 = "ty_term (map_of (parameters (detype_ac a))) d2.constT"
+
     have tyt_om: "\<forall>x. ?tyt x \<noteq> None \<longrightarrow> ?tyt2 x = Some \<omega>" using t_ac_tyt by simp
+    from assms have wfa: "wf_action_schema a" using wf_D(7) by simp
 
-    from assms have wfa: "wf_action_schema a" using wf_domain wf_domain_def by simp
-    from assms have "distinct (map fst (parameters a))" using wfa wf_ac_expanded by metis
-    hence c1: "distinct (map fst (parameters ?a2))" using t_ents_dis detype_ac_def by auto
-    from assms have "wf_fmla ?tyt (ac_pre a)" using wfa wf_ac_expanded by metis
+    from assms have "distinct (map fst (parameters a))" using wfa wf_ac_alt by metis
+    hence c1: "distinct (map fst (parameters ?a2))" using t_ents_dis detype_ac_alt by auto
+
+    from assms have "wf_fmla ?tyt (ac_pre a)" using wfa wf_ac_alt by metis
     hence c2b: "d2.wf_fmla ?tyt2 (ac_pre a)" using tyt_om t_fmla_wf by blast
-    from assms have "wf_effect ?tyt (ac_eff a)" using wfa wf_ac_expanded by metis
-    hence "d2.wf_effect ?tyt2 (ac_eff a)"
-      using tyt_om ast_domain.wf_effect.simps t_eff_wf detype_ac_def by blast
-    hence c3: "d2.wf_effect ?tyt2 (ac_eff ?a2)" using detype_ac_def by simp
-
-    have "wf_action_params a" using restrD restrict_dom_def assms by simp
+    have "wf_action_params a" using restr_D(2) assms by simp
     note c2a = t_param_precond_wf[OF this]
-    from c2a c2b have c2: "d2.wf_fmla ?tyt2 (ac_pre ?a2)" by (simp add: detype_ac_def)
+    from c2a c2b have c2: "d2.wf_fmla ?tyt2 (ac_pre ?a2)" by (simp add: detype_ac_alt)
 
-    from c1 c2 c3 show ?thesis using d2.wf_ac_expanded by simp
+    from assms have "wf_effect ?tyt (ac_eff a)" using wfa wf_ac_alt by metis
+    hence "d2.wf_effect ?tyt2 (ac_eff a)"
+      using tyt_om ast_domain.wf_effect.simps t_eff_wf detype_ac_alt by blast
+    hence c3: "d2.wf_effect ?tyt2 (ac_eff ?a2)" using detype_ac_alt by simp
+
+    from c1 c2 c3 show ?thesis using d2.wf_ac_alt by simp
   qed
 
   lemma (in restr_domain2) t_acs_wf:
     shows "(\<forall>a\<in>set (map detype_ac (actions D)). d2.wf_action_schema a)"
-    using detype_dom_def wf_dom_def t_ac_wf by simp
+    using detype_dom_def wf_D t_ac_wf by simp
 
-text \<open> init / goal \<close>
+(* --------------------------------------------------------------------- *)
 
-lemma (in wf_ast_problem) t_init_dis: "distinct (init P2)"
-proof -
-  have "init P2 = supertype_facts (objects P) @ supertype_facts (consts D) @ (init P)"
-    using detype_prob_def by simp
-  show ?thesis sorry
-qed
+text \<open> init / goal \<close> (* TODO maybe move elsewhere *)
+
+  abbreviation (input) get_t :: "type \<Rightarrow> name" where
+    "get_t T \<equiv> hd (primitives T)"
+  lemma "get_t (Either ts) = hd ts" by simp
+
+  lemma "distinct (supertypes_of t)" using reachable_dis by metis
+
+  lemma superfacts_for_cond:
+    assumes "single_type T"
+    shows "supertype_facts_for (n, T) =
+        map (Atom \<circ> (\<lambda>p. predAtm p [n])) (supertype_preds (get_t T))"
+    using assms type.collapse supertype_facts_for.simps(1)
+    using list.sel(1) list_decomp_1 sorry
+
+  lemma a: "distinct (supertype_preds t)"
+    using supertype_preds_def reachable_dis pred_for_type_dis by metis
+
+  lemma b:
+    assumes "distinct preds"
+    shows "distinct (map (\<lambda>p. predAtm p args) preds)"
+  proof -
+    have "inj (\<lambda>p. predAtm p args)" 
+      by (simp add: inj_def)
+    thus ?thesis
+      using assms map_inj_dis by fastforce
+  qed
+
   
-lemma (in wf_ast_problem2) t_init_wf:
-  "p2.wf_world_model (set (init P2))"
-  sorry
+
+  lemma c: "distinct (supertype_facts_for (n, Either [t]))"
+  proof -
+    have dis: "distinct (map (\<lambda>p. predAtm p [n]) (supertype_preds t))"
+      using a b by auto
+    have inj: "inj Atom" by (simp add: inj_def)
+    note map_inj_dis[OF dis inj]
+    thus ?thesis by simp
+  qed
+
+  lemma c': "single_type T \<Longrightarrow> distinct (supertype_facts_for (n, T))"
+    using c
+    by (metis list_decomp_1 type.collapse)
+
+
+  lemma d:
+    assumes "n \<noteq> m"
+    shows "set (supertype_facts_for (n, Either [t1])) \<inter> set (supertype_facts_for (m, Either [t2])) = {}"
+    (is "?l \<inter> ?r = {}")
+  proof -
+    have "x \<noteq> y" if "x \<in> ?l \<and> y \<in> ?r" for x y
+    proof -
+      from that obtain k where 1: "x = Atom k" "atom.arguments k = [n]" by auto
+      from that obtain g where 2: "y = Atom g" "atom.arguments g = [m]" by auto
+      from 1 2 show ?thesis using assms by fastforce
+    qed
+    thus ?thesis by auto
+  qed
+
+  lemma d': assumes "n \<noteq> m" "single_type T1" "single_type T2"
+    shows "set (supertype_facts_for (n, T1)) \<inter> set (supertype_facts_for (m, T2)) = {}"
+    using assms d
+    by (metis list_decomp_1 type.collapse)
+  
+  lemma d'': assumes "n \<notin> fst ` set cs" "single_types cs" "single_type T"
+    shows "set (supertype_facts_for (n, T)) \<inter> set (supertype_facts cs) = {}"
+    (is "?l \<inter> ?r = {}")
+    using d' sorry
+
+  lemma "\<lbrakk>length (primitives T) = 1; \<And>t. P (Either [t]) t\<rbrakk> \<Longrightarrow> P T (hd (primitives T))"
+    by (metis list.sel(1) list_decomp_1 type.collapse)
+
+  lemma h:
+    assumes
+      "x \<in> set (supertype_facts_for (n, Either [t]))"
+    shows "\<exists> st. st \<in> set (supertypes_of t) \<and>
+                 x = Atom (predAtm (pred_for_type st) [n])"
+  proof -
+    from assms obtain st where
+      stin: "st \<in> set (supertypes_of t)" and
+      x: "x = Atom (predAtm (pred_for_type st) [n])"
+      by (auto simp add: supertype_preds_def)
+    thus ?thesis by simp
+  qed
+
+  lemma h':
+    assumes
+      "x \<in> set (supertype_facts_for (n, T))" "single_type T"
+    shows "\<exists> st. st \<in> set (supertypes_of (hd (primitives T))) \<and>
+                 x = Atom (predAtm (pred_for_type st) [n])"
+    using assms
+    by (simp add: h superfacts_for_cond)
+
+  lemma q: "pred ` set (predicates D) \<inter> pred ` (set type_preds) = {}"
+    by (metis Int_commute dt_preds_ids image_set tps_dt_preds_disj)
+
+  lemma (in wf_ast_problem) r: assumes "x \<in> set (init P)"
+    shows "\<exists>p \<in> pred ` set (predicates D). \<exists>args. x = Atom (predAtm p args)"
+  proof -
+    from assms have 1: "wf_fmla_atom objT x"
+      by (meson wf_world_model_def wf_P)
+    then obtain a vs where 2: "x = Atom (predAtm a vs)"
+      using wf_fmla_atom.elims(2) by blast
+    from 1 2 have "wf_pred_atom objT (a, vs)" by simp
+    hence "sig a \<noteq> None"
+      by (metis option.simps(4) wf_pred_atom.simps)
+    hence "a \<in> pred ` set (predicates D)"
+      by (metis image_eqI option.exhaust predicate_decl.sel(1) sig_some)
+    from this 2 show ?thesis by simp
+  qed
+
+  lemma i:
+  assumes "single_types ents"
+  shows "\<forall>x \<in> set (supertype_facts ents). \<exists> t a. x = Atom (predAtm (pred_for_type t) a)"
+  using assms h' supertype_facts_def by fastforce
+
+  lemma e:
+  assumes "distinct (map fst objs)" "single_types objs"
+  shows "distinct (supertype_facts objs)"
+  using assms proof (induction objs)
+    case (Cons ob obs)
+    hence notin: "fst ob \<notin> fst ` set obs" by auto
+    hence int: "set (supertype_facts_for ob) \<inter> set (supertype_facts obs) = {}"
+      using d''[OF notin] Cons.prems by fastforce
+    from Cons have dis2: "distinct (supertype_facts obs)" by simp
+    from c' Cons.prems have "distinct (supertype_facts_for ob)" by auto
+    thus ?case using int dis2 supertype_facts_def by simp
+  qed (simp add: supertype_facts_def)
+
+  (* doesn't really matter because if I can't prove it, I'll just throw remdups at it *)
+  lemma (in restr_problem) t_init_dis: "distinct (init P2)"
+  proof -
+    have 0: "init P2 = supertype_facts (objects P) @ supertype_facts (consts D) @ (init P)"
+      using detype_prob_def by simp
+    have 1: "distinct (map fst ((consts D) @ (objects P)))" using wf_P by fastforce
+    have 2: "single_types (consts D @ objects P)"
+      using single_t_objs by auto
+    from 1 2 have "distinct (supertype_facts (consts D @ objects P))" using e by simp
+    hence dis1: "distinct (supertype_facts (objects P) @ supertype_facts (consts D))"
+      using supertype_facts_def by auto
+    have dis2: "distinct (init P)" using wf_P by auto
+    have int: "set (supertype_facts (consts D @ objects P)) \<inter> set (init P) = {}" sorry
+
+    from dis1 dis2 int 0 supertype_facts_def show ?thesis by auto
+  qed
+
+  lemma (in wf_ast_domain) supertypes_listed:
+    assumes "t \<in> set type_names"
+    shows "set (supertypes_of t) \<subseteq> set type_names"
+  proof -
+    (* why is this so tedious? *)
+    have 1: "snd ` set (types D) \<subseteq> set type_names"
+      using wf_D wf_types_def type_names_set by simp
+  
+    have "set (supertypes_of t) \<subseteq> insert t (snd ` set (types D))"
+      using reachable_set by simp
+    also have "... \<subseteq> insert t (set type_names)" using 1 by blast
+    also have "... \<subseteq> set type_names" using assms by simp
+  
+    ultimately show ?thesis by blast
+  qed
+
+  thm wf_ast_domain2.type_pred_sig
+
+  (* TODO simplify *)
+  lemma (in wf_ast_problem2) super_facts_for_wf:
+    assumes "length (primitives T) = 1"
+      "(n, T) \<in> set (consts D @ objects P)"
+    shows "\<forall>\<phi> \<in> set (supertype_facts_for (n, T)). d2.wf_fmla_atom p2.objT \<phi>"
+  proof
+    fix \<phi> assume phi_in: "\<phi> \<in> set (supertype_facts_for (n, T))"
+
+    from assms obtain t where t: "T = Either [t]"
+      by (metis list_decomp_1 type.collapse)
+    hence "supertype_facts_for (n, T) = map (Atom \<circ> (\<lambda>p. predAtm p [n])) (supertype_preds t)"
+      by simp
+    from this phi_in obtain sp where
+      sp_in: "sp \<in> set (supertype_preds t)" and
+      phi: "\<phi> = Atom (predAtm sp [n])" by auto
+    from this obtain st where
+      sp: "sp = pred_for_type st" and
+      st_in: "st \<in> set (supertypes_of t)" using supertype_preds_def by auto
+
+    from assms(2) have "wf_type T" using wf_DP by auto
+    hence tin: "t \<in> set type_names" using wf_type_iff_listed t by simp
+    from this st_in have st_in': "st \<in> set type_names" using supertypes_listed by blast
+    from tin have "\<forall>st \<in> set (supertypes_of t). st \<in> set type_names"
+      using supertypes_listed by blast
+
+    note type_pred_sig[OF st_in']
+    hence sp_sig: "d2.sig sp = Some [\<omega>]" using sp by simp
+
+    from assms(2) have "objT n \<noteq> None" using objT_Some by simp
+    hence n_obj: "p2.objT n = Some \<omega>" using t_objT_Some by simp
+
+    from phi show "d2.wf_fmla_atom p2.objT \<phi>"
+      using sp_sig n_obj d2.is_of_type_def by fastforce
+  qed
+
+  lemma (in wf_ast_problem2) super_facts_wf:
+    assumes "single_types ents"
+      "set ents \<subseteq> set (consts D @ objects P)"
+    shows "\<forall>\<phi> \<in> set (supertype_facts ents). d2.wf_fmla_atom p2.objT \<phi>"
+    using assms supertype_facts_def super_facts_for_wf by fastforce
+
+  lemma (in restr_problem2) t_init_wf:
+    "p2.wf_world_model (set (init P2))"
+  proof -
+    have 1: "\<forall>c. (objT c \<noteq> None) \<longrightarrow> (p2.objT c = Some \<omega>)" using t_objT_Some by simp
+    have "\<forall>\<phi> \<in> set (init P). wf_fmla_atom objT \<phi>"
+      using wf_world_model_def wf_P by simp
+    hence c1: "\<forall>\<phi> \<in> set (init P). p2.wf_fmla_atom p2.objT \<phi>"
+      using t_fmla_atom_wf 1 by (auto simp add: detype_prob_def)
+
+    have c23: "\<forall>\<phi> \<in> set (supertype_facts (consts D @ objects P)). d2.wf_fmla_atom p2.objT \<phi>"
+      using super_facts_wf single_t_objs by blast
+    
+    from c1 c23 show ?thesis
+      using detype_prob_def supertype_facts_def p2.wf_world_model_def by auto
+  qed
 
 
 text \<open> major\<close>
@@ -835,7 +1143,7 @@ text \<open> major\<close>
     have c1: "d2.wf_types" using d2.wf_types_def detype_dom_def by simp
     note c2 = t_preds_dis
     note c3 = t_preds_wf
-    have "distinct (map fst (consts D))" using wf_dom_def by simp
+    have "distinct (map fst (consts D))" using wf_D by simp
     hence c4: "distinct (map fst (detype_ents(consts D)))"
       by (simp add: t_ents_dis)
     have c5: "(\<forall>(n,T)\<in>set (detype_ents (consts D)). d2.wf_type T)"
@@ -845,14 +1153,14 @@ text \<open> major\<close>
     note c7 = t_acs_wf
   
     from c1 c2 c3 c4 c5 c6 c7 show ?thesis
-      using d2.wf_domain_def detype_dom_def by simp
+      using d2.wf_domain_def detype_dom_def by auto
   qed
 
   theorem (in restr_problem2) detype_prob_wf:
     shows "p2.wf_problem"
   proof -
     note c1 = detype_dom_wf
-    have "distinct (map fst (objects P) @ map fst (consts D))" using wf_prob_def by simp
+    have "distinct (map fst (objects P) @ map fst (consts D))" using wf_P by simp
     hence c2: "distinct (map fst (detype_ents (objects P)) @ map fst (detype_ents (consts D)))"
       using t_ents_names by metis
     have c3: "\<forall>(n, y)\<in>set (objects P2). p2.wf_type y"
@@ -861,7 +1169,7 @@ text \<open> major\<close>
     note c5 = t_init_wf
   
     have c6a: "\<forall>e. objT e \<noteq> None \<longrightarrow> p2.objT e = Some \<omega>" using t_objT_Some by simp
-    have c6b: "wf_fmla objT (goal P2)" using detype_prob_def wf_prob_def by simp
+    have c6b: "wf_fmla objT (goal P2)" using detype_prob_def wf_P by simp
     have c6: "p2.wf_fmla p2.objT (goal P2)"
       using t_fmla_wf[OF c6a c6b] detype_prob_def by simp
     from c1 c2 c3 c4 c5 c6 show ?thesis
@@ -922,13 +1230,61 @@ text \<open> Supertype Enumeration \<close>
       t \<in> set (supertypes_of ot))"
     using assms is_obj_of_type_def single_of_type_iff by auto
 
+
+
 end
+
+text \<open> major \<close>
+
+context restr_problem2
+begin
+
+abbreviation "super_facts \<equiv> supertype_facts (objects P @ consts D)"
+abbreviation "sf_substate \<equiv> set super_facts"
+
+lemma t_init_substate: "set (init P2) = sf_substate \<union> set (init P)" using detype_prob_def supertype_facts_def by auto
+
+lemma t_init_disj: "sf_substate \<inter> set (init P) = {}" sorry
+
+lemma t_substate_static: "sf_substate \<subseteq> s \<Longrightarrow> sf_substate \<subseteq> p2.execute_plan_action \<pi> s"
+  oops
+
+
+(* left direction not true, use \uplus instead *)
+lemma t_exec_equiv: "execute_plan_action \<pi> s = s' \<longleftrightarrow> p2.execute_plan_action \<pi> (sf_substate \<union> s) = sf_substate \<union> s'"
+  oops
+
+
+lemma "s \<inter> t = {} \<Longrightarrow> s' = s \<longleftrightarrow> (s' \<inter> t = {} \<and> s' \<union> t = s \<union> t)" by auto
+
+lemma x3:
+  assumes "sf_substate \<inter> s' = {}"
+  shows "plan_action_path (set (init P)) \<pi>s s' \<longleftrightarrow> p2.plan_action_path (set (init P2)) \<pi>s (sf_substate \<union> s')"
+  using assms
+proof (induction \<pi>s arbitrary: s')
+  case Nil
+  have "plan_action_path (set (init P)) Nil s' \<longleftrightarrow> s' = set (init P)" by simp
+  also have "... \<longleftrightarrow> s' \<union> sf_substate = set (init P) \<union> sf_substate" using t_init_disj sorry
+  have "\<And>s''. plan_action_path (set (init P2)) Nil s'' \<longleftrightarrow> s'' = set (init P2) \<union> sf_substate"
+    using t_init_substate by force
+  oops
+
+lemma x2: "s \<^sup>c\<TTurnstile>\<^sub>= goal P \<longleftrightarrow> sf_substate \<union> s \<^sup>c\<TTurnstile>\<^sub>= goal P2"
+  oops
+
+lemma "valid_plan \<pi>s \<Longrightarrow> p2.valid_plan \<pi>s"
+  apply (induction \<pi>s)
+  oops
+
+
+end
+
 
 (* ---------------------- Future Milestones ------------------------- *)
 
 (* type normalization correct w.r.t. execution*)
 
-lemma (in restr_problem) "valid_plan \<pi> \<Longrightarrow> ast_problem.valid_plan detype_prob \<pi>"
-  oops
+
+
 
 end
